\documentclass{article}
\usepackage{breqn}
\begin{document}
\begin{dgroup*}
\begin{dmath*}
\tau_{{\mathrm{bar}}}=0
\end{dmath*}
\begin{dmath*}
A=0
\end{dmath*}
\begin{dmath*}
a=0
\end{dmath*}
\begin{dmath*}
\mathrm{bar}=0
\end{dmath*}
\begin{dmath*}
\mathrm{bar}_{2^{3}}=0
\end{dmath*}
\begin{dmath*}
\mathrm{foo}_{1}=0
\end{dmath*}
\begin{dmath*}
\mathrm{gamma}=\Gamma\left( t \right)
\end{dmath*}
\begin{dmath*}
\mathrm{uf0}=\mathrm{uf0}()
\end{dmath*}
\begin{dmath*}
s=\left(7\right)!
\end{dmath*}
\begin{dmath*}
r=\left( 1 \right)\%
\end{dmath*}
\begin{dmath*}
q=\arctan\left(\infty \right)
\end{dmath*}
\begin{dmath*}
\mathrm{polygamma}=\psi^{\left(0\right)}\left( t \right)
\end{dmath*}
\begin{dmath*}
p=\arcsin\left( 1 \right)
\end{dmath*}
\begin{dmath*}
o=\arccos\left( 0 \right)
\end{dmath*}
\begin{dmath*}
n=\cos\left(\pi \right)
\end{dmath*}
\begin{dmath*}
m=\ln\left( e \right)
\end{dmath*}
\begin{dmath*}
\mathrm{foo}=\mathrm{bar}
\end{dmath*}
\begin{dmath*}
d=\frac{ t }{1}
\end{dmath*}
\begin{dmath*}
c=\mathrm{}( t )
\end{dmath*}
\begin{dmath*}
\mathrm{catching}=\exp\left(\left(\mathrm{Loans}+ t -\left(\mathrm{foo}+\tau_{{\mathrm{bar}}}\right)\right)\times b\right)
\end{dmath*}
\begin{dmath*}
\mathrm{Repay}=\frac{\mathrm{foo}+\tau_{{\mathrm{bar}}}}{\mathrm{Loans}+ t }
\end{dmath*}
\begin{dmath*}
g=\left| t \right|\times \mathrm{frac}( t )\times \left\lfloor t \right\rfloor)\times \theta\left(- t \right)\times \theta\left( t \right)\times \theta\left(\mathrm{Repay}- t \right)\times \theta\left(- t \right)+\delta\left( t \right)\times \theta\left( t \right)+\delta\left( t \right)\times \theta\left(\mathrm{Repay}- t \right)+\delta\left( t -\mathrm{Repay}\right)
\end{dmath*}
\begin{dmath*}
l=\left(1-\theta\left(0.5-\max\left(\theta\left(\theta\left(\mathrm{Repay}- t \right)+\delta\left( t -\mathrm{Repay}\right)-0.5\right),\theta\left(\theta\left( t \right)\right)\right)\right)\right)+\theta\left(\theta\left( t \right)-0.5\right)+\theta\left(\theta\left( t \right)-0.5\right)
\end{dmath*}
\begin{dmath*}
k=\theta\left(\theta\left( t \right)-0.5\right)\theta\left(\theta\left( t \right)+\delta\left( t \right)-0.5\right)+0+0
\end{dmath*}
\begin{dmath*}
h=\delta\left( t \right)+\delta\left( t \right)+\delta\left(g- t \right)
\end{dmath*}
\begin{dmath*}
i=\min\left(g, t \right)
\end{dmath*}
\begin{dmath*}
j=\max\left(g, t \right)+\max\left( t ,0\right)+\min\left( t ,0\right)+\min\left( t ,0\right)+\max\left( t ,0\right)
\end{dmath*}
\begin{dmath*}
\mathrm{uf1}=\mathrm{uf1(x)}\left(j\right)
\end{dmath*}
\begin{dmath*}
\mathrm{uf2}=\mathrm{uf2(x,y)}\left(j,l\right)
\end{dmath*}
\begin{dmath*}
F(0)=0
\end{dmath*}
\begin{dmath*}
\frac{ d F}{dt} =\mathrm{foo}\times  t \end{dmath*}
\begin{dmath*}
\mathrm{Loans}(0)=0
\end{dmath*}
\begin{dmath*}
\frac{ d \mathrm{Loans}}{dt} =A+\mathrm{Repay}-\mathrm{catching}\end{dmath*}
\begin{dmath*}
b(0)=-0
\end{dmath*}
\begin{dmath*}
\frac{ d b}{dt} =\mathrm{Repay}-\mathrm{catching}\end{dmath*}
\begin{dmath*}
\mathrm{fooey}(0)=0
\end{dmath*}
\begin{dmath*}
\frac{ d \mathrm{fooey}}{dt} =\left(a+b\right)^{\log_{d}\left(c\right)}\end{dmath*}
\begin{dmath*}
\mathrm{int}(0)=0
\end{dmath*}
\begin{dmath*}
\frac{ d \mathrm{int}}{dt} =\tanh\left(\cosh\left(\sinh\left(\tan\left(\cos\left(\sin\left(\ln\left(\sqrt{ t }\right)\right)\right)\right)\right)\right)\right)\end{dmath*}
\begin{dmath*}
\mathrm{int1}(0)=0
\end{dmath*}
\begin{dmath*}
\frac{ d \mathrm{int1}}{dt} =\arctan\left(\arccos\left(\arcsin\left( t \right)\right)\right)\end{dmath*}
\end{dgroup*}
\end{document}
